Spec_ra progress

theories/app_rel_logic/spec_ra.v
@@ -8,20 +8,20 @@ From iris.proofmode Require Import proofmode.
 From clutch.common Require Import language ectxi_language spec_update.
 From clutch.prob_lang Require Import locations lang.
 
-Definition specN := nroot .@ "spec".
+(* Definition specN := nroot .@ "spec". *)
 
 (* We will through [spec_interp] tie the exact state (both heap and tapes) to a
    fragmental view that lives in [spec_ctx]; from here we will give meaning to
    the usual [spec] resource and points-to connectivs *)
 Definition progUR : ucmra := optionUR (exclR exprO).
-Definition cfgO : ofe := prodO exprO stateO.
-Definition cfgUR : ucmra := optionUR (exclR cfgO).
+(* Definition cfgO : ofe := prodO exprO stateO. *)
+(* Definition cfgUR : ucmra := optionUR (exclR cfgO). *)
 
 (** The CMRA for the spec [cfg]. *)
 Class specGS Σ := CfgSG {
   (* the instances we need for [spec_interp] *)
-  specGS_interp_inG :: inG Σ (authUR cfgUR);
-  specGS_interp_name : gname;
+  (* specGS_interp_inG :: inG Σ (authUR cfgUR); *)
+  (* specGS_interp_name : gname; *)
 
   (* the instances we need for [spec_ctx] *)
   specGS_prog_inG :: inG Σ (authR progUR);
@@ -35,63 +35,80 @@ Class specGS Σ := CfgSG {
 
 Section resources.
   Context `{!specGS Σ}.
-
-  Definition spec_interp_auth (ρ : cfg) : iProp Σ :=
-    own specGS_interp_name (● (Excl' ρ : cfgUR)).
-  Definition spec_interp_frag (ρ : cfg) : iProp Σ :=
-    own specGS_interp_name (◯ (Excl' ρ : cfgUR)).
-
-  Lemma spec_interp_auth_frag_agree ρ ρ' :
-    spec_interp_auth ρ -∗ spec_interp_frag ρ' -∗ ⌜ρ = ρ'⌝.
-  Proof.
-    iIntros "Ha Hf".
-    iDestruct (own_valid_2 with "Ha Hf") as
-      %[Hexcl ?]%auth_both_valid_discrete.
-    rewrite Excl_included in Hexcl.
-    by apply leibniz_equiv in Hexcl.
-  Qed.
-
-  Lemma spec_interp_update ρ'' ρ ρ' :
-    spec_interp_auth ρ -∗ spec_interp_frag ρ' ==∗ spec_interp_auth ρ'' ∗ spec_interp_frag ρ''.
-  Proof.
-    iIntros "Ha Hf".
-    iDestruct (spec_interp_auth_frag_agree with "Ha Hf") as %->.
-    iMod (own_update_2 with "Ha Hf") as "[Ha Hf]".
-    { by eapply auth_update, option_local_update,
-      (exclusive_local_update _ (Excl ρ'')). }
-    by iFrame.
-  Qed.
-
-  Definition spec_prog_auth (e : expr) : iProp Σ :=
+  Definition spec_prog_auth e :=
     own specGS_prog_name (● (Excl' e : progUR)).
-  Definition spec_prog_frag (e : expr) : iProp Σ :=
-    own specGS_prog_name (◯ (Excl' e : progUR)).
-
-  Lemma spec_prog_auth_frag_agree e e' :
-    spec_prog_auth e -∗ spec_prog_frag e' -∗ ⌜e = e'⌝.
-  Proof.
-    iIntros "Ha Hf".
-    iDestruct (own_valid_2 with "Ha Hf") as
-      %[Hexcl ?]%auth_both_valid_discrete.
-    rewrite Excl_included in Hexcl.
-    by apply leibniz_equiv in Hexcl.
-  Qed.
-
-  Lemma spec_prog_update e'' e e' :
-    spec_prog_auth e -∗ spec_prog_frag e' ==∗ spec_prog_auth e'' ∗ spec_prog_frag e''.
-  Proof.
-    iIntros "Ha Hf".
-    iDestruct (spec_prog_auth_frag_agree with "Ha Hf") as %->.
-    iMod (own_update_2 with "Ha Hf") as "[Ha Hf]".
-    { by eapply auth_update, option_local_update,
-      (exclusive_local_update _ (Excl e'')). }
-    by iFrame.
-  Qed.
-
   Definition spec_heap_auth `{specGS Σ} :=
     @ghost_map_auth _ _ _ _ _ specGS_heap specGS_heap_name 1.
   Definition spec_tapes_auth `{specGS Σ} :=
     @ghost_map_auth _ _ _ _ _ specGS_tapes specGS_tapes_name 1.
+
+  Definition spec_interp_auth (ρ : cfg) : iProp Σ :=
+    spec_prog_auth (ρ.1) ∗
+    spec_heap_auth (ρ.2.(heap)) ∗
+    spec_tapes_auth (ρ.2.(tapes))
+  .
+
+  Definition spec_prog_frag (e : expr) : iProp Σ :=
+    own specGS_prog_name (◯ (Excl' e : progUR)).
+
+  
+  (* Definition spec_interp_frag (ρ : cfg) : iProp Σ := *)
+  (*   own specGS_interp_name (◯ (Excl' ρ : cfgUR)). *)
+
+  Lemma spec_interp_auth_frag_agree_expr e1 σ1 e2  :
+    spec_interp_auth (e1, σ1) -∗ spec_prog_frag e2 -∗ ⌜e1 = e2⌝.
+  Proof.
+    iIntros "[Ha _] Hf".
+    iDestruct (own_valid_2 with "Ha Hf") as
+      %[Hexcl ?]%auth_both_valid_discrete.
+    rewrite Excl_included in Hexcl.
+    by apply leibniz_equiv in Hexcl.
+  Qed.
+
+  Lemma spec_interp_update e1 σ1 e2 e3 :
+    spec_interp_auth (e1, σ1) -∗ spec_prog_frag e2 ==∗ spec_interp_auth (e3, σ1) ∗ spec_prog_frag e3.
+  Proof.
+    iIntros "Ha Hf".
+    iDestruct (spec_interp_auth_frag_agree_expr with "Ha Hf") as %->.
+    iDestruct "Ha" as "[Ha Hb]".
+    iMod (own_update_2 with "Ha Hf") as "[Ha Hf]".
+    { by eapply auth_update, option_local_update,
+        (exclusive_local_update _ (Excl e3)). }
+    by iFrame.
+  Qed.
+
+  Definition spec_auth_spec : spec _ _ := Spec spec_interp_auth.
+
+  (* Definition spec_prog_auth (e : expr) : iProp Σ := *)
+  (*   own specGS_prog_name (● (Excl' e : progUR)). *)
+  (* Definition spec_prog_frag (e : expr) : iProp Σ := *)
+  (*   own specGS_prog_name (◯ (Excl' e : progUR)). *)
+
+  (* Lemma spec_prog_auth_frag_agree e e' : *)
+  (*   spec_prog_auth e -∗ spec_prog_frag e' -∗ ⌜e = e'⌝. *)
+  (* Proof. *)
+  (*   iIntros "Ha Hf". *)
+  (*   iDestruct (own_valid_2 with "Ha Hf") as *)
+  (*     %[Hexcl ?]%auth_both_valid_discrete. *)
+  (*   rewrite Excl_included in Hexcl. *)
+  (*   by apply leibniz_equiv in Hexcl. *)
+  (* Qed. *)
+
+  (* Lemma spec_prog_update e'' e e' : *)
+  (*   spec_prog_auth e -∗ spec_prog_frag e' ==∗ spec_prog_auth e'' ∗ spec_prog_frag e''. *)
+  (* Proof. *)
+  (*   iIntros "Ha Hf". *)
+  (*   iDestruct (spec_prog_auth_frag_agree with "Ha Hf") as %->. *)
+  (*   iMod (own_update_2 with "Ha Hf") as "[Ha Hf]". *)
+  (*   { by eapply auth_update, option_local_update, *)
+  (*     (exclusive_local_update _ (Excl e'')). } *)
+  (*   by iFrame. *)
+  (* Qed. *)
+
+  (* Definition spec_heap_auth `{specGS Σ} := *)
+  (*   @ghost_map_auth _ _ _ _ _ specGS_heap specGS_heap_name 1. *)
+  (* Definition spec_tapes_auth `{specGS Σ} := *)
+  (*   @ghost_map_auth _ _ _ _ _ specGS_tapes specGS_tapes_name 1. *)
 
 End resources.
 
@@ -118,39 +135,39 @@ Notation "l ↪ₛ{# q } v" := (l ↪ₛ{ DfracOwn q } v)%I
 Notation "l ↪ₛ v" := (l ↪ₛ{ DfracOwn 1 } v)%I
   (at level 20, format "l  ↪ₛ  v") : bi_scope.
 
-Section spec_ctx.
-  Context `{!invGS_gen HasNoLc Σ, !specGS Σ}.
+(* Section spec_ctx. *)
+(*   Context `{!invGS_gen HasNoLc Σ, !specGS Σ}. *)
 
-  Definition spec_inv : iProp Σ :=
-    (∃ ρ e σ n,
-        spec_interp_frag ρ ∗
-        ⌜pexec n ρ (e, σ) = 1%R⌝ ∗
-        spec_prog_auth e ∗
-        spec_heap_auth σ.(heap) ∗
-        spec_tapes_auth σ.(tapes))%I.
+(*   Definition spec_inv : iProp Σ := *)
+(*     (∃ ρ e σ n, *)
+(*         spec_interp_frag ρ ∗ *)
+(*         ⌜pexec n ρ (e, σ) = 1%R⌝ ∗ *)
+(*         spec_prog_auth e ∗ *)
+(*         spec_heap_auth σ.(heap) ∗ *)
+(*         spec_tapes_auth σ.(tapes))%I. *)
 
-  Definition spec_ctx : iProp Σ :=
-    inv specN spec_inv.
+(*   Definition spec_ctx : iProp Σ := *)
+(*     inv specN spec_inv. *)
 
-  Global Instance spec_ctx_persistent : Persistent spec_ctx.
-  Proof. apply _. Qed.
+(*   Global Instance spec_ctx_persistent : Persistent spec_ctx. *)
+(*   Proof. apply _. Qed. *)
 
-  Definition refines_right K (e : expr) := (spec_ctx ∗ ⤇ fill K e)%I.
+(*   Definition refines_right K (e : expr) := (spec_ctx ∗ ⤇ fill K e)%I. *)
 
-  Lemma refines_right_bind K' K e :
-    refines_right K' (fill K e) ≡ refines_right (K ++ K') e.
-  Proof. rewrite /refines_right /=. by rewrite fill_app. Qed.
+(*   Lemma refines_right_bind K' K e : *)
+(*     refines_right K' (fill K e) ≡ refines_right (K ++ K') e. *)
+(*   Proof. rewrite /refines_right /=. by rewrite fill_app. Qed. *)
 
-End spec_ctx.
+(* End spec_ctx. *)
 
-Ltac iAsimpl :=
-  repeat match goal with
-  | |- context [ (⤇ ?e)%I ] => progress (
-    let e' := fresh in evar (e':expr);
-    assert (e = e') as ->; [unfold e'; reflexivity|];
-    unfold e'; clear e')
-  | |- context [ WP ?e @ _ {{ _ }}%I ] => progress (
-    let e' := fresh in evar (e':expr);
-    assert (e = e') as ->; [unfold e'; reflexivity|];
-    unfold e'; clear e')
-    end.
+(* Ltac iAsimpl := *)
+(*   repeat match goal with *)
+(*   | |- context [ (⤇ ?e)%I ] => progress ( *)
+(*     let e' := fresh in evar (e':expr); *)
+(*     assert (e = e') as ->; [unfold e'; reflexivity|]; *)
+(*     unfold e'; clear e') *)
+(*   | |- context [ WP ?e @ _ {{ _ }}%I ] => progress ( *)
+(*     let e' := fresh in evar (e':expr); *)
+(*     assert (e = e') as ->; [unfold e'; reflexivity|]; *)
+(*     unfold e'; clear e') *)
+(*     end. *)
